Especificaciones/Auxiliar/NaturalsFacts.dfy
@@ -1,53 +1,82 @@
+/*
+    File explanation
+        The main goal of this file is to provide lemmas about operations with natural numbers that, although trivially true, need explicit invoking  in order for some properties to verify 
+    
+    Predicates: 
+        None
 
+    Functions:
+        None
 
-//Used locally by atMostOneLessThanHalfImplies2Aproximated
-lemma MultiplyingByNaturals(a: nat, b: nat, c: nat)
+    Lemmas:
+        -LessThanOrEqualMultiplication: If a number is greater or equal than another, the result of multiplying the first by a thrid number is greater or equal than the result of multiplying the other by that same third number
+
+    Methods:
+        None
+
+    Imported elements
+        None
+*/
+
+//If a number is greater or equal than another, 
+//the result of multiplying the first by a thrid number is greater or equal than the result of multiplying the other by that same third number
+//Used locally by LessThanDivision
+//Used in BinPacking2AproximatedAux.dfy by AtMostOneLessThanHalfImplies2AproximatedCalc and AtMostOneLessThanHalfImplies2Aproximated
+lemma LessThanOrEqualMultiplication(a: nat, b: nat, c: nat)
 requires a <= b
 ensures a * c <= b * c
 { }
 
-//Used locally by dividingByNaturals
-lemma MultiplyingByNaturals2(a: nat, b: nat, c: nat)
-requires a < b
-requires c > 0
-ensures a * c < b * c
-{ }
-
-//Used locally by atMostOneLessThanHalfImplies2Aproximated
-lemma DividingByNaturals(a: nat, b: nat, c: nat)
+//Same idea as the lemma above, but now the implication goes in the other direction, for it to hold, the third number must be greater than 0
+//Used in BinPacking2AproximatedAux by atMostOneLessThanHalfImplies2AproximatedCalc
+//Used in EnvasadoPropertirs by EachBinHasLesserThanEWeight
+lemma LessThanDivision(a: nat, b: nat, c: nat)
 requires a * c < b * c
 requires c > 0
 ensures a < b
 {
     if a >= b {
-        MultiplyingByNaturals(b, a, c);
+        LessThanOrEqualMultiplication(b, a, c);
+        assert false;
     }
 }
 
-//Used locally by atMostOneLessThanHalfImplies2Aproximated
+//The product is commutative
+//Used in BinPacking2AproximatedAux by AtMostOneLessThanHalfImplies2AproximatedCalc
 lemma CommutativeProduct(a: nat, b: nat, c: nat)
 ensures a * b * c == a * c *b
 { }
 
-//Used locally by atMostOneLessThanHalfImplies2Aproximated
+//It is possible to use the distributivity property to simplify additions and multiplications
+//Used in BinPacking2AproximatedAux by LowerBoundSum
 lemma Distributivity(a: nat, b: nat, c: nat)
 ensures (a - b) * c + b * c == a * c 
 { }
 
-//Used locally by atMostOneLessThanHalfImplies2Aproximated
+//It is possible to use common factor to simplify additions and multiplications
+//Used in BinPacking2AproximatedAux by LowerBoundSum
 lemma ProductSimplification(a: nat, b: nat)
 ensures a * b + b == (a + 1) * b
 { }
 
-//Used locally by multisetsMoreThanHalf
+//The result of a substraction of naturals is a smaller number when the substracted element is not 0
+//Used in BinPacking2AproximatedAux by multisetsMoreThanHalf
 lemma IsSmallerThan(a: nat, b: nat, c: nat)
 requires a == b - c 
 requires c > 0
 ensures a < b  
 { }
 
-//Used locally by eachBinHasLesserThanEWeight
-lemma lessThanWithMultiplication(a: nat, b: nat, c: nat)
-requires a <= c 
-ensures a * b <= c * b 
+//////////////////////////////////////////////////
+//               Currently Unused               //
+//////////////////////////////////////////////////
+/*
+//If a number is greater or equal than another, 
+//the result of multiplying the first by a thrid number is greater or equal than the result of multiplying the other by that same third number
+//The third number must be strictly greater than 0 for this to hold
+lemma LessThanMultiplication(a: nat, b: nat, c: nat)
+requires a < b
+requires c > 0
+ensures a * c < b * c
 { }
+*/
