Especificaciones/Clique/Clique.dfy
@@ -10,7 +10,7 @@ include "../Auxiliar/Graph.dfy"
 */
 
 predicate isClique(g: Graph, I: set<Node>)
-    requires isValidGraph(g)
+    requires isValidGraph(g) 
 {
     I <= g.0 && forall a, b: Node | a in I && b in I && a != b :: {a, b} in g.1
 }
