Especificaciones/Clique/CliqueOpt.dfy
@@ -11,7 +11,7 @@ include "Clique.dfy"
             From Clique.dfy
             -isClique
 */ 
-
+ 
 //Decission problem: returns true if there exists a clique with size k or larger
 ghost predicate CliqueDecissionProblem(g: Graph, k: nat)
     requires isValidGraph(g)
